@prefix cs: <https://data.surroundaustralia.com/def/prof-roles> .
@prefix rdf:  <http://www.w3.org/1999/02/22-rdf-syntax-ns#> .
@prefix rdfs: <http://www.w3.org/2000/01/rdf-schema#> .
@prefix owl:  <http://www.w3.org/2002/07/owl#> .
@prefix xsd:  <http://www.w3.org/2001/XMLSchema#> .
@prefix sdo: <https://schema.org/> .
@prefix skos: <http://www.w3.org/2004/02/skos/core#> .
@prefix reg:  <http://purl.org/linked-data/registry#> .
@prefix dcterms:  <http://purl.org/dc/terms/> .
@prefix vann: <http://purl.org/vocab/vann/> .
@prefix : <https://data.surroundaustralia.com/def/prof-roles/> .


<https://data.surroundaustralia.com/def/prof-roles> 
    a owl:Ontology , skos:ConceptScheme;
    skos:prefLabel "PROF Roles Vocabulary"@en ;
    skos:definition """This vocabulary is a flat - no hierarchy - listing of the roles for people and organisations defined within the ISO standard 19135 "Geographic information â€” Procedures for item registration ISO/DIS 19135-1" https://www.iso.org/standard/54721.html."""@en ;
    owl:versionIRI <https://data.surroundaustralia.com/def/prof-roles/1.0> ;
    owl:versionInfo "1.0"@en ;
    dcterms:contributor <https://orcid.org/0000-0002-8742-7730>;
    vann:preferredNamespaceUri "https://data.surroundaustralia.com/def/prof-roles/"^^xsd:string ;
    dcterms:creator <http://orcid.org/0000-0002-8742-7730> ;
    vann:preferredNamespacePrefix "prof-roles"@en ;
    dcterms:publisher <https://linked.data.gov.au/org/surround> ;
    rdfs:seeAlso <https://github.com/surroundaustralia/prof-roles> ;
    dcterms:issued "2021-11-13"^^xsd:date ;
    dcterms:modified "2021-11-13"^^xsd:date ;
    dcterms:rights "(c) SURROUND Australia Pty Ltd, 2021"@en ;
    dcterms:created "2021-11-13"^^xsd:date ;
    dcterms:source "https://www.w3.org/TR/dx-prof/"^^xsd:anyURI ;
    skos:hasTopConcept 
        <http://www.w3.org/ns/dx/prof/role/constraints> ,
        <http://www.w3.org/ns/dx/prof/role/example> ,
        <http://www.w3.org/ns/dx/prof/role/guidance> ,
        <http://www.w3.org/ns/dx/prof/role/mapping> ,
        :repository ,
        <http://www.w3.org/ns/dx/prof/role/schema> ,
        <http://www.w3.org/ns/dx/prof/role/specification> ,
        <http://www.w3.org/ns/dx/prof/role/validation> ,
        <http://www.w3.org/ns/dx/prof/role/vocabulary> ;
.

<https://linked.data.gov.au/def/surround>
    a sdo:Organization ;
    sdo:name "SURROUND Australia Pty Ltd" ;
    sdo:url "https://surroundaustralia.com"^^xsd:anyURI ;
.

<https://orcid.org/0000-0002-8742-7730>
    a sdo:Person ;
    sdo:honorificPrefix "Dr" ;
    sdo:name "Nicholas J. Car" ;
    sdo:email "nicholas.car@surroundaustralia.com"^^xsd:anyURI ;
    sdo:affiliation <https://linked.data.gov.au/org/surround> ;
.

<http://www.w3.org/ns/dx/prof/role/constraints>
    a skos:Concept ;
    rdfs:isDefinedBy <http://www.w3.org/ns/dx/prof/role> ;
    skos:prefLabel "Constraints"@en ;
    skos:definition "Descriptions of obligations, limitations or extensions that the profile defines"@en ;
    skos:inScheme cs: ;
    skos:scopeNote "Use this Role when you want to indicate the constraints that the associated Profile imposes on top of base specifications"@en ;
    skos:topConceptOf cs: ;
.

<http://www.w3.org/ns/dx/prof/role/example>
    a skos:Concept ;
    rdfs:isDefinedBy <http://www.w3.org/ns/dx/prof/role> ;
    skos:prefLabel "Example"@en ;
    skos:definition "Sample instance data conforming to the profile"@en ;
    skos:inScheme cs: ;
    skos:scopeNote "Use this Role when you want to provide instances of data conforming to the profile to inform users"@en ;
    skos:topConceptOf cs: ;
.

<http://www.w3.org/ns/dx/prof/role/guidance>
    a skos:Concept ;
    rdfs:isDefinedBy <http://www.w3.org/ns/dx/prof/role> ;
    skos:prefLabel "Guidance"@en ;
    skos:definition "Documents, in human-readable form, how to use the profile"@en ;
    skos:inScheme cs: ;
    skos:scopeNote "	Many existing profiles treat their human-readable forms (PDF documents etc.) as authoritative. This role is suggestive of non-authoritativeness. For a role for a human-readable resource that is authoritative, see Specification"@en ;
    skos:topConceptOf cs: ;
.

<http://www.w3.org/ns/dx/prof/role/mapping>
    a skos:Concept ;
    rdfs:isDefinedBy <http://www.w3.org/ns/dx/prof/role> ;
    skos:prefLabel "Mapping"@en ;
    skos:definition "Describes conversions between two Standards"@en ;
    skos:inScheme cs: ;
    skos:editorialNote "Changed word Specifications to Standards in definition compared with PROF"@en ;
    skos:topConceptOf cs: ;
.

:repository
    a skos:Concept ;
    rdfs:isDefinedBy <https://data.surroundaustralia.com/def/prof-roles> ;
    skos:prefLabel "Repository"@en ;
    skos:definition "A system used to store all, or many, of the Profile's parts"@en ;
    skos:inScheme cs: ;
    skos:scopeNote "Commonly used to indicate an online version control repository."@en ;
    skos:topConceptOf cs: ;
.

<http://www.w3.org/ns/dx/prof/role/schema>
    a skos:Concept ;
    rdfs:isDefinedBy <http://www.w3.org/ns/dx/prof/role> ;
    skos:prefLabel "Schema"@en ;
    skos:altLabel 
        "Shape"@en , 
        "Structure"@en ; 
    skos:definition "Machine-readable structural descriptions of data defined by the profile"@en ;
    skos:inScheme cs: ;
    skos:scopeNote ""@en ;
    skos:topConceptOf cs: ;
.

<http://www.w3.org/ns/dx/prof/role/specification>
    a skos:Concept ;
    rdfs:isDefinedBy <http://www.w3.org/ns/dx/prof/role> ;
    skos:prefLabel "Specification"@en ;
    skos:definition "Defining the profile in human-readable form"@en ;
    skos:inScheme cs: ;
    skos:scopeNote "This role indicates authoritativeness. For a role for a human-readable resource that is not authoritative, see Guidance"@en ;
    skos:topConceptOf cs: ;
.

<http://www.w3.org/ns/dx/prof/role/validation>
    a skos:Concept ;
    rdfs:isDefinedBy <http://www.w3.org/ns/dx/prof/role> ;
    skos:prefLabel "Validation"@en ;
    skos:definition "Supplies instructions about how to verify conformance of data to the profile"@en ;
    skos:inScheme cs: ;
    skos:scopeNote "This role implies inclusion or import of inherited constraints"@en ;
    skos:topConceptOf cs: ;
.

<http://www.w3.org/ns/dx/prof/role/vocabulary>
    a skos:Concept ;
    rdfs:isDefinedBy <http://www.w3.org/ns/dx/prof/role> ;
    skos:prefLabel "Vocabulary"@en ;
    skos:definition "Defines terms used in the profile specification"@en ;
    skos:inScheme cs: ;
    skos:topConceptOf cs: ;
.
